Crypto.AEAD top-level verifies, modulo documented assumptions

examples/low-level/crypto/Crypto.AEAD.Lemmas.fst
@@ -50,7 +50,15 @@ let find_append (#i:id) (#r:rid) (d:domain i) (s1:Seq.seq (PRF.entry r i)) (s2:S
            (ensures (find (Seq.append s1 s2) d == find s2 d))
    = admit() //NS: boring
 
-assume val to_seq_temp: #a:Type -> b:Buffer.buffer a -> l:UInt32.t{v l <= Buffer.length b} -> ST (Seq.seq a)
+#set-options "--initial_ifuel 0 --max_ifuel 0 --initial_fuel 2 --max_fuel 2"
+let find_singleton (#rgn:region) (#i:id) (e:PRF.entry rgn i) (x:PRF.domain i) 
+    : Lemma (if is_entry_domain x e then PRF.find (Seq.create 1 e) x == Some e.range
+	     else PRF.find (Seq.create 1 e) x == None)
+    = ()	     
+
+#reset-options "--initial_ifuel 0 --max_ifuel 0 --initial_fuel 2 --max_fuel 2"
+assume //NS: boring, this should be in the buffer library
+val to_seq_temp: #a:Type -> b:Buffer.buffer a -> l:UInt32.t{v l <= Buffer.length b} -> ST (Seq.seq a)
   (requires (fun h -> Buffer.live h b))
   (ensures  (fun h0 r h1 -> h0 == h1 /\ Buffer.live h1 b /\ r == Buffer.as_seq h1 b))
 ////////////////////////////////////////////////////////////////////////////////
@@ -293,7 +301,7 @@ val pre_refines_to_refines: (i:id) -> (st:state i Writer) -> (nonce: Cipher.iv (
 	              let c, tag = SeqProperties.split c_tagged len in
 		      let ad = Buffer.as_seq h aad in
   		      safeId i ==> 
-			(none_above ({iv=nonce; ctr=0ul}) st.prf h0 /\
+			(none_above ({iv=nonce; ctr=ctr_0 i}) st.prf h0 /\
    			 pre_refines_one_entry i st nonce len plain cipher h0 h /\
 			 mac_refines i st nonce aad plain cipher h)))
             (ensures (let mac_rgn = st.prf.mac_rgn in
@@ -593,17 +601,22 @@ let frame_counterblocks_snoc i t x k len completed_len plain cipher h0 h1 =
   assert (Seq.equal (as_bytes p) (as_bytes p0));
   assert (p == p0); 
   let initial_x = {x with ctr=ctr_0 i +^ 1ul} in
-  (* let initial_blocks = counterblocks i t.mac_rgn initial_x len 0 completed_len p0 c0 in *)
-  (* let final_blocks = counterblocks i t.mac_rgn initial_x len 0 (completed_len + next) p c in *)
-  (* let plain_last = Plain.slice p completed_len (completed_len + next) in *)
-  (* let cipher_last = Seq.slice c completed_len (completed_len + next) in *)
-  (* let last_entry = PRF.Entry ({x with ctr=UInt32.uint_to_t k}) *)
-  (* 		   (PRF.OTP (UInt32.uint_to_t next) plain_last cipher_last) in *)
-  (* let from = (v initial_x.ctr - 1) * v (PRF.blocklen i) in *)
   counterblocks_snoc  #i t.mac_rgn initial_x k len next completed_len p c;
   counterblocks_slice #i t.mac_rgn initial_x len 0 completed_len p c;
   counterblocks_slice #i t.mac_rgn initial_x len 0 completed_len p0 c0
 
+#set-options "--initial_ifuel 1 --max_ifuel 1 --initial_fuel 2 --max_fuel 2"
+let invert_contains_plain_and_cipher_block   (#i:id) (#r:rid) (#l:u32{l <=^ PRF.blocklen i})
+					     (x:domain i{safeId i /\ ctr_0 i <^ x.ctr})
+					     (plain:plain i (v l))
+					     (cipher:lbytes (v l))
+					     (b:PRF.entry r i)
+    : Lemma (requires (contains_plain_block x plain (Seq.create 1 b) /\
+		       contains_cipher_block (v l) x cipher (Seq.create 1 b)))
+            (ensures (b == PRF.Entry #r #i x (PRF.OTP l plain cipher)))
+    = ()
+
+#reset-options "--initial_fuel 0 --max_fuel 0 --initial_ifuel 0 --max_ifuel 0 --z3timeout 400"
 val extending_counter_blocks: #i:id -> (t:PRF.state i) -> (x:domain i{ctr_0 i <^ x.ctr}) ->
 			     len:nat{len <> 0 /\ safelen i len (ctr_0 i +^ 1ul)} -> 
 			     (completed_len:nat{completed_len < len /\
@@ -628,6 +641,7 @@ val extending_counter_blocks: #i:id -> (t:PRF.state i) -> (x:domain i{ctr_0 i <^
 		    none_above x t h0 /\
 		    (safeId i ==> 
 		       (let r = itable i t in
+			let blocks_1 = HS.sel h1 (PRF.itable i t) in
 		        h0 `HS.contains` r /\
 			HS.sel h0 t.table == 
 			  Seq.append (HS.sel h_init t.table)
@@ -635,9 +649,8 @@ val extending_counter_blocks: #i:id -> (t:PRF.state i) -> (x:domain i{ctr_0 i <^
 						 len 0 completed_len
 						 (Plain.sel_plain h0 (u len) plain)
 						 (Buffer.as_seq h0 cipher)) /\
-	                ( match find_otp #t.mac_rgn #i (HS.sel h1 t.table) x with
-			  | Some (OTP l' p c) -> u l = l' /\ p == sel_plain h1 (u l) plain_hd /\ c == sel_bytes h1 (u l) cipher_hd
-			  | None   -> False )))))
+                        contains_plain_block x (sel_plain h1 (u l) plain_hd) blocks_1 /\
+			contains_cipher_block l x (sel_bytes h1 (u l) cipher_hd) blocks_1))))
           (ensures (let remaining_len = len - completed_len in
 		    let l = minNat remaining_len (v (PRF.blocklen i)) in
 		    let completed_len' = completed_len + l in
@@ -669,7 +682,6 @@ val extending_counter_blocks: #i:id -> (t:PRF.state i) -> (x:domain i{ctr_0 i <^
    = Seq.append init (snoc (counterblocks ..) last_entry)  //by a standard snoc/append lemma
    = Seq.append init final_blocks                          //by frame_counterblocks_snoc
 *)
-
 let extending_counter_blocks #i t x len completed_len plain cipher h0 h1 h_init
   = if safeId i
     then begin
@@ -678,6 +690,10 @@ let extending_counter_blocks #i t x len completed_len plain cipher h0 h1 h_init
 	 let r1 = HS.sel h1 r in 
  	 let suffix = SeqProperties.last r1 in
 	 assert (Seq.equal r1 (SeqProperties.snoc r0 suffix));
+	 assert (PRF.find r0 x == None);
+	 find_append x r0 (Seq.create 1 suffix);
+	 find_singleton suffix x;
+	 assert (PRF.find r1 x == Some suffix.range);    
 	 let p = Plain.sel_plain h1 (u len) plain in
 	 let c = Buffer.as_seq h1 cipher in
 	 let remaining_len = len - completed_len in
@@ -685,12 +701,13 @@ let extending_counter_blocks #i t x len completed_len plain cipher h0 h1 h_init
 	 let plain_last = Plain.slice p completed_len (completed_len + next) in
 	 let cipher_last = Seq.slice c completed_len (completed_len + next) in
 	 let last_entry = PRF.Entry #t.mac_rgn #i x (PRF.OTP (UInt32.uint_to_t next) plain_last cipher_last) in
-	 let plain_last' = 
+	 let plain_last' =
 	     Plain.sel_plain h1 (u next) (Plain.sub plain (u completed_len) (u next)) in
-         let cipher_last' = 
+         let cipher_last' =
 	     sel_bytes h1 (u next) (Buffer.sub cipher (u completed_len) (u next)) in
 	 assert (Seq.equal (Plain.as_bytes #i #next plain_last) (Plain.as_bytes #i #next plain_last'));
 	 assert (Seq.equal cipher_last cipher_last');
+	 invert_contains_plain_and_cipher_block #i #t.mac_rgn #(u next) x plain_last cipher_last suffix;
 	 assert (suffix == last_entry);
 	 frame_counterblocks_snoc i t x (v x.ctr) len completed_len plain cipher h0 h1
     end
